theories/L/Complexity/Reductions/TMGenNP/LM_to_mTM.v
@@ -15,7 +15,7 @@ Check LMtoTM.M.
 
 From Undecidability Require Import LSum.
 
-From Undecidability Require Import CompCode. 
+From Undecidability Require Import CompCode.
 
 Import ProgrammingTools.
 
@@ -23,32 +23,32 @@ Module TrueOrDiverge.
   Import TM.TM ProgrammingTools CaseList CaseBool Code.Decode Code.DecodeList.
 
   Section sec.
-  Variable (n:nat) (sig : finType) (M' : pTM sig bool n).
+    Variable (n:nat) (sig : finType) (M' : pTM sig bool n).
 
-  Definition M := If M' Nop Diverge.
+    Definition M := If M' Nop Diverge.
 
-  Lemma Realises R' (H' : M' ⊨ R'):
-    M ⊨ (fun tin out => R' tin (true,snd out)).
-  Proof.
-    eapply Realise_monotone.
-    { eapply If_Realise. eassumption. now TM_Correct. now apply Diverge_Realise. }
-    hnf. intros x [[] y]. intros [H|H].
-    -cbn in H. destruct H as (?&?&<-). easy. 
-    -exfalso. cbn in H. firstorder.
-  Qed.
+    Lemma Realises R' (H' : M' ⊨ R'):
+      M ⊨ (fun tin out => R' tin (true,snd out)).
+    Proof.
+      eapply Realise_monotone.
+      { eapply If_Realise. eassumption. now TM_Correct. now apply Diverge_Realise. }
+      hnf. intros x [[] y]. intros [H|H].
+      -cbn in H. destruct H as (?&?&<-). easy.
+      -exfalso. cbn in H. firstorder.
+    Qed.
 
-  Import TM.
-  
-  Lemma TerminatesIn R' (HR' : M' ⊨ R') T' (HT' : projT1 M' ↓ T'):
-    projT1 M ↓ (fun tin k => T' tin (k-1) /\ 0 < k /\ forall tout, ~ R' tin (false,tout)).
-  Proof.
-    eapply TerminatesIn_monotone.
-    { eapply If_TerminatesIn. 1,2:eassumption. now TM_Correct. now apply Canonical_TerminatesIn. }
-    intros tin [] (HTtin&Hfalse). easy. 
-    do 2 eexists;repeat simple apply conj. eassumption.
-    2:{ intros ? ? ?. destruct b. reflexivity. now exfalso. }
-    nia.
-  Qed.
+    Import TM.
+
+    Lemma Terminates R' (HR' : M' ⊨ R') T' (HT' : projT1 M' ↓ T'):
+      projT1 M ↓ (fun tin k => T' tin (k-1) /\ 0 < k /\ forall tout, ~ R' tin (false,tout)).
+    Proof.
+      eapply TerminatesIn_monotone.
+      { eapply If_TerminatesIn. 1,2:eassumption. now TM_Correct. now apply Canonical_TerminatesIn. }
+      intros tin [] (HTtin&Hfalse). easy.
+      do 2 eexists;repeat simple apply conj. eassumption.
+      2:{ intros ? ? ?. destruct b. reflexivity. now exfalso. }
+      nia.
+    Qed.
   End sec.
 End TrueOrDiverge.
 
@@ -57,142 +57,213 @@ Arguments LMtoTM.M : clear implicits.
 
 
 (*move*)
+Lemma initValue_sizeOfTape (sig sigX X : Type) (cX : codable sigX X) (I : Retract sigX sig) (x : X):
+  sizeOfTape (initValue cX I x) = size x + 2.
+Proof.
+  cbn. autorewrite with list. cbn. now unfold size.
+Qed.
+
+
+Lemma initRight_sizeOfTape sig :
+  sizeOfTape (initRight sig) = 1.
+Proof.
+  cbn. nia.
+Qed.
+
+Module M.
+  Section M.
+    Arguments LMtoTM.M : clear implicits.
+    Definition sig := (finType_CS (HaltingProblem.sigStep + sigList bool)).
+
+    Definition sig__reg : registered sig := LFinType.registered_finType.
+
+    Definition Retr1 : Retract _ sig := (Retract_inl _ (Retract_id _)).
+    Definition Retr2 : Retract _ sig := (Retract_inr _ (Retract_id _)).
+
+    Let n := 11.
+    Definition M : pTM _ _ n := TrueOrDiverge.M (LMtoTM.M sig Retr1 Retr2).
+    Definition ts__start : Pro -> tapes (sig^+) (n-1) :=
+      (fun P => CodeTM.initValue _ (@LMtoTM.retr__pro _ Retr1) P ::: Vector.const (CodeTM.initRight _) (n-2)).
+
+    Definition Rel : pRel (sig ^+) unit 11 :=
+      fun tin _ =>
+        forall P t__cert, tin = t__cert:::ts__start P
+                   -> exists bs : list bool,
+            t__cert ≃(Retr2) bs /\
+            (exists (sigma' : LM_heap_def.state) (k : nat), evaluatesIn LM_heap_def.step k (initLMGen P (compile (enc (rev bs)))) sigma').
+
+
+    Definition Realises :
+      M ⊨
+        (fun tin _ =>
+           forall P t__cert, tin = t__cert:::ts__start P
+                      -> exists bs : list bool,
+               t__cert ≃(Retr2) bs /\
+               (exists (sigma' : LM_heap_def.state) (k : nat), evaluatesIn LM_heap_def.step k (initLMGen P (compile (enc (rev bs)))) sigma')).
+    Proof.
+      unfold M. eapply Realise_monotone.
+      1:now eapply TrueOrDiverge.Realises, LMtoTM.Realises.
+      intros ? out H P t__cert ->. hnf in H|-*. specialize (H P).
+      apply H.
+      -apply CodeTM.initValue_contains.
+      -intros ?. cbn - [Vector.const]. rewrite Vector.const_nth. now apply CodeTM.initRight_isRight.
+    Qed.
+
+    Definition time := @f__UpToC _ _ (projT1 (@LMtoTM._Terminates sig Retr1 Retr2)).
+
+    Definition Terminates :
+      projT1 M ↓ (fun tin k => 0 < k /\
+                            exists P k__LM t__cert (bs : list bool),
+                              tin = t__cert ::: ts__start P
+                              /\ t__cert ≃(Retr2) bs
+                              /\ (exists sigma' : LM_heap_def.state, evaluatesIn LM_heap_def.step k__LM (initLMGen P (compile (enc (rev bs)))) sigma')
+                              /\ time (k__LM, sizeOfmTapes tin) <= k-1).
+    Proof.
+      unfold M. eapply TerminatesIn_monotone.
+      {eapply TrueOrDiverge.Terminates. now apply LMtoTM.Realises. apply LMtoTM.Terminates. }
+      intros tin k (HkPos&P&k__LM&t__cert&bs&->&Ht__cert&HLM&Htime). unfold LMtoTM.Ter.
+      split.
+      2:{ split. easy. unfold LMtoTM.Rel. intros _ H. eapply (H P).
+          -apply CodeTM.initValue_contains.
+          -intros ?. cbn - [Vector.const]. rewrite Vector.const_nth. now apply CodeTM.initRight_isRight.
+          -eauto.
+      }
+      exists P,k__LM.
+      repeat simple apply conj.
+      -apply CodeTM.initValue_contains.
+      -intros ?. cbn - [Vector.const]. rewrite Vector.const_nth. now apply CodeTM.initRight_isRight.
+      -right. exists bs;split. all:easy.
+      -eassumption.
+    Qed.
+  End M.
+
+    
+  Lemma sizeStart t__cert P:
+    sizeOfmTapes (t__cert ::: M.ts__start P)
+    = max (sizeOfTape t__cert) (size P + 2).
+  Proof.
+    unfold sizeOfmTapes. rewrite Vector.fold_left_right_assoc_eq. 2:nia. cbn - [Vector.const initValue initRight].
+    rewrite <- Vector.fold_left_right_assoc_eq.  2:nia.
+    set (tmp:= VectorDef.const _ _). change (VectorDef.fold_left _ _ _) with (sizeOfmTapes tmp).
+    rewrite initValue_sizeOfTape.
+    replace (sizeOfmTapes tmp) with 1. nia.
+    subst tmp. clear.
+    unfold sizeOfmTapes. rewrite Vector.fold_left_right_assoc_eq. 2:nia.
+    generalize 8 as x. induction x.
+    -reflexivity.
+    -cbn in *. now rewrite <- IHx.
+  Qed.
+    
+    
+End M.
+
+(*move*)
+Lemma size_rev X {_:registered X} (xs : list X): L.size (enc (rev xs)) = L.size (enc xs).
+Proof.
+  rewrite !size_list,map_rev,<- sumn_rev. easy.
+Qed.
+
+
+(*move*)
 Lemma uniform_confluent_confluent (X : Type) (R : X -> X -> Prop):
   uniform_confluent R -> confluent R.
 Proof.
-  intros H x y y' Hy Hy'. apply ARS.star_pow in Hy as (?&Hy). apply ARS.star_pow in Hy' as (?&Hy'). 
+  intros H x y y' Hy Hy'. apply ARS.star_pow in Hy as (?&Hy). apply ARS.star_pow in Hy' as (?&Hy').
   edestruct parametrized_confluence as (?&?&z&?&?&?&?&?).
   eassumption. exact Hy. exact Hy'. exists z. split;eapply pow_star. all:easy.
-Qed. 
-  
-Lemma LMGenNP_to_TMGenNP_mTM :
-  {sig : finType &
-   {n:nat &
-    {R__sig : registered sig &
-     {M : mTM sig (S n) & 
-          restrictBy (LMHaltsOrDiverges (list bool)) (LMGenNP (list bool)) ⪯p (restrictBy (HaltsOrDiverges_fixed_mTM M) (TMGenNP_fixed_mTM M))}}}}.
+Qed.
+
+
+Lemma LMGenNP_to_TMGenNP_mTM (_ : registered M.sig):
+  restrictBy (LMHaltsOrDiverges (list bool)) (LMGenNP (list bool)) ⪯p (restrictBy (HaltsOrDiverges_fixed_mTM (projT1 M.M)) (TMGenNP_fixed_mTM (projT1 M.M))).
 Proof.
-  evar (sig : finType). evar (tau : finType). evar (n:nat).
-  unshelve epose (_:mTM tau (S n)) as M.
-  { unshelve notypeclasses refine (projT1 ( (*TrueOrDiverge.M*) (@LMtoTM.M sig _ _))).
-    2:now notypeclasses refine (Retract_inl _ (Retract_id _)).
-    now notypeclasses refine (Retract_inr _ (Retract_id _)).
-  } cbn in M.
-  unshelve eexists _,n,_,M.
-  now apply LFinType.registered_finType.
-  set (Retr1 := Retract_inr _ _) in M.
-  set (Retr2 := Retract_inl _ _) in M.
+  evar (f__size:nat -> nat).
+  Import Datatypes.Lists Datatypes.LBool.
+  enough (Hcert_f__size : forall maxSize (bs : list bool) sig R, size (enc bs) <= maxSize -> sizeOfTape (initValue (sig:=sig) _ R bs) <= f__size maxSize).
 
-  evar (R__Pro: Retract Alphabets.sigPro sig). unfold sig in tau. cbn in tau. 
-
-  evar (ts__start:Pro -> tapes tau (S (n-1))).
-  [ts__start]: refine (fun (P :Pro) => CodeTM.initValue _ R__Pro P ::: Vector.const (CodeTM.initRight _) (n-1)).
   
-  evar (tmp2:Type). evar (f__steps:tmp2).
-  evar (tmp3:Type). evar (f__size:tmp3).
-  eapply reducesPolyMO_intro_restrictBy with
-      (f:=fun '(P,maxSize,steps) => (ts__start P,f__size maxSize,f__steps steps P maxSize));subst tmp2;subst tmp3.
+  evar (f__steps:nat * Pro * nat -> nat).
+  enough (Hf__steps : forall steps P maxSize t__cert k__LM,
+             sizeOfTape t__cert <= f__size maxSize
+             -> k__LM <= steps ->
+             M.time (k__LM, sizeOfmTapes (t__cert ::: M.ts__start P)) <= f__steps (steps,P,maxSize)).
+
+  
+  
+  eapply @reducesPolyMO_intro_restrictBy with
+      (f:=fun '(P,maxSize,steps) => (M.ts__start P,f__size maxSize,S (f__steps (steps,P,maxSize)))).
+  2:intros [[P maxSize] steps] H; split.
+  2:{ hnf in H|-*. destruct H as ((s&->&s__proc)&HsmallCert&Hk).
+      intros t__cert' k res' HM.
+      specialize (M.Realises HM) as H'. hnf in H'. specialize H' with (1:=eq_refl) as (bs'&Hbs'&(sigma'&k__LM'&HbsRed')).
+      specialize HsmallCert with (1:=HbsRed') as (bs&res__LM&Hbs&HbsRed&Hter__LM). clear HM k res' t__cert' bs' Hbs' sigma' k__LM' HbsRed'.
+      apply star_pow in HbsRed as (k__LM&HbsRed).
+      assert (Hk__LM : k__LM <= steps).
+      { eapply Hk. exact Hbs. split. all:eassumption. }
+      edestruct M.Terminates as (conf'&eq).
+      2:{ eexists (initValue _ _ (rev bs)),_. split. 2:eassumption. eapply Hcert_f__size. rewrite size_rev. easy. }
+      split. now clear;Lia.nia.
+      eexists _,_,_,(rev bs).
+      repeat simple apply conj.
+      1:now reflexivity.
+      1:now apply initValue_contains.
+      2:{
+        unshelve erewrite (_ : forall x, S x - 1 = x). 1:now clear;nia.
+        apply Hf__steps. 2:eassumption. eapply Hcert_f__size.  rewrite size_rev. easy.
+      }
+      rewrite rev_involutive. unfold evaluatesIn;eauto.
+  }
+  3:{ intros steps P maxSize t__cert k__LM Hsize Hk__LM.
+      rewrite M.sizeStart.
+      unfold M.time.
+      rewrite UpToC_le.
+      rewrite !Hk__LM. clear Hk__LM k__LM.
+      rewrite !Hsize. clear Hsize t__cert.
+      [f__steps]:refine (fun '(steps,P,maxSize) => _). unfold f__steps. reflexivity.
+  }
+  3:{ intros maxSize bs sig R Hsize. rewrite initValue_sizeOfTape. 
+      
+      specialize @correct__leUpToC with (l:=M_Boollist_to_Enc.BoollistToEnc.boollist_size) (x:=bs) as ->.
+      rewrite <- size_list_enc_r in Hsize. rewrite Hsize. 
+      [f__size]:refine (fun n => _). subst f__size;cbn beta. reflexivity.
+  }
+
   2:{
-    intros [[P maxSize] steps] H. split.
-    { hnf in H|-*. destruct H as ((s&Hs&s__proc)&HsmallCert&Hk).
-      intros t__cert Hsize k conf__res HM.
-      
-      apply LMtoTM.Realises in HM as HM__sound. hnf in HM__sound. specialize (HM__sound P).
-      Tactic Notation "mp" hyp(L) "as" ident(H) :=
-        lazymatch type of L with
-          ?t -> _ => 
-          assert (H:t);[ |
-                         specialize (L H)]
-        end.
-      mp HM__sound as HMP.
-      { cbn. unfold R__Pro. apply initValue_contains. }
-      mp HM__sound as HMright.
-      { intros. cbn - [Vector.const]. rewrite Vector.const_nth. apply initRight_isRight. }
-      
-      specialize LMtoTM.Terminates with (sig:=_) (retr__LAM:=Retr1) (retr__list:=Retr2) as HM__terminate.
-      set (M' := projT1 _) in HM__terminate at 1; replace M' with M in *;[ | unfold M,M';reflexivity];clear M'.
-      hnf in HM__terminate.
-
-      specialize HM__terminate as (conf' & HM__terminate).
-      2:{ erewrite loop_injective with (b:=conf__res). 3:exact HM__terminate. 2:eassumption.
-          eassumption.
-      }
-      cbn -[ts__start] in HMP.
-      hnf.
-      exists P. 
-      set (t__M := f__UpToC _) at 1.
-      cut (forall steps__LM, steps__LM <= steps -> 
-                      t__M (steps__LM, sizeOfmTapes (t__cert ::: ts__start P)) <= f__steps steps P maxSize).
-      {
-        intros Hmono.
-        destruct (projT2 _) eqn:Heqcase in HM__sound.
-        2:{ eexists 0. repeat simple apply conj.
-            -exact HMP.
-            -exact HMright.
-            -left. split. 2:easy. eassumption.
-            -apply Hmono. clear;nia. 
-        }
-        edestruct HM__sound as (bs&?&?&k0&?).
-        cbn in H.
-        specialize sizeOfTape_tape_contains_size with (1:=tape_contains_contains_size H) as Hsize_bs.
-        set (tmp := sizeOfTape _) in Hsize,Hsize_bs. rewrite <- Hsize_bs in Hsize at 1. clear Hsize_bs tmp.
-
-        { (*specialize HsmallCert with (1:=H0) as (cert'&sigma'&Hcert'size&(k'&Hcert'R)%(proj1 (@ARS.star_pow _ _ _ _))). *)
-         eexists k0. repeat simple apply conj.
-          -exact HMP.
-          -exact HMright.
-          -right. eauto.
-          -apply Hmono.
-           (*specialize HsmallCert with (1:=H0) as (cert'&sigma'&Hcert'size&Hcert'R).
-           replace x with sigma' in *.
-           2:{
-             eapply ARS.unique_normal_forms with (R:= LM_heap_def.step).
-             -eapply uniform_confluent_confluent,functional_uc, LM_heap_def.step_functional.
-             -destruct H0 as (H0'&?). apply pow_star,star_ecl in H0'. apply star_ecl in Hcert'R. rewrite <- H0',<-Hcert'R.
-           destruct (HsmallCert _ _ _H0) *)
-           eapply Hk. 2:eassumption.
-           Set Nested Proofs Allowed.
-           (*move*)
-           Lemma size_rev X {_:registered X} (xs : list X): L.size (enc (rev xs)) = L.size (enc xs).
-           Proof.
-             rewrite !size_list,map_rev,<- sumn_rev. easy.
-           Qed.
-
-           rewrite size_rev.
-           
-           (*move*)
-           Lemma Lsize_list_bool_le:
-             (fun (bs : list bool) => L.size (enc bs)) <=c (fun bs => length bs + 1).
-           Admitted.
-           Lemma length_le_TMsize_list_bool:
-             (fun (bs : list bool) => length bs + 1) <=c size.
-           Admitted.
-           specialize @correct__leUpToC with (l:=Lsize_list_bool_le) (x:=bs) as ->.
-           specialize @correct__leUpToC with (l:=length_le_TMsize_list_bool) (x:=bs) as ->.
-           rewrite Hsize.
-           rewrite <- mult_assoc_reverse.
-           set (c:= c__leUpToC * c__leUpToC).
-           enough (Hdiv:f__size maxSize <= maxSize / (c+1)).
-           { unshelve erewrite (_ : c <= c +1) at 1. clear;nia.
-             rewrite Hdiv,Nat.mul_div_le. 2:clear;nia. reflexivity.
-           }
-           [f__size]:refine (fun n => _). subst f__size;cbn beta. reflexivity.
-        }
-      }
-      (* TODO: instantiate using monotonic property? *)
-      Import String. instantiate (f__steps := TODO ("above, and abstract important properties")).
-      admit. 
-    }
-    (* TODO: We might canc opy some reasoning from the first part down here*)
-    (* TODO: do we need HsmallCert? *)
-    destruct H as ((s&->&s__proc)&HsmallCert&Hk).
+    destruct H as ((s&->&s__proc)&HsmallCert&Hsmallk).
     unfold LMGenNP, TMGenNP_fixed_mTM.
     split.
-    -intros (cert & HcertSize & sigma & k' &Hk' &HR'). admit.
-     
-    -admit. 
+    -intros (cert' & HcertSize' & sigma'' & k' &Hk' &HR').
+     edestruct M.Terminates with (k:= S (f__steps (steps,compile s,maxSize))) as (tout&Hout).
+     { split. easy. eexists _,_,_,(rev cert'). rewrite rev_involutive. repeat simple apply conj.
+       1:reflexivity.
+       2:eexists;exact HR'.
+       1:now apply initValue_contains.
+       { unshelve erewrite (_ : forall x, S x - 1 = x). 1:now clear;nia.
+         apply Hf__steps. 2:eassumption.
+         eapply Hcert_f__size. now rewrite size_rev.
+       }
+     }
+     do 2 eexists.
+     2:{
+       eexists. eassumption. }
+     eapply Hcert_f__size. now rewrite size_rev.
+    -intros (t__cert&Hsize_t__cert&(res&Hres)).
+     specialize (M.Realises Hres) as H'. hnf in H'. specialize H' with (1:=eq_refl) as (bs'&Hbs'&(sigma'&k__LM'&HbsRed')).
+      specialize HsmallCert with (1:=HbsRed') as (bs&res__LM&Hbs&HbsRed&Hter__LM). clear Hres bs' Hbs' sigma' k__LM' HbsRed'.
+      apply star_pow in HbsRed as (k__LM&HbsRed).
+      assert (Hk__LM : k__LM <= steps).
+      { eapply Hsmallk. exact Hbs. split. all:eassumption. }
+      exists bs. repeat simple apply conj. 1:easy. unfold evaluatesIn; eauto 10.
   }
-  admit.
+  {
+    clear Hf__steps Hcert_f__size.
+    enough (polyTimeComputable f__steps).
+    enough (polyTimeComputable f__size).
+
+    - admit. (*TODO: Lemmas for PolyTimeComputable, See CanEnumTerm.v*)
+    - admit.
+    - admit.
+  }
 Admitted.
 
 Print Assumptions LMGenNP_to_TMGenNP_mTM.
